rec <-> word

src/Rec.v
@@ -1,10 +1,6 @@
 Require Import Arith List String Omega. 
 Require Import Pred.
 Require Import Word.
-Require Import Prog.
-Require Import Hoare.
-Require Import SepAuto.
-Require Import BasicProg.
 
 Import ListNotations.
 Open Scope string_scope.
@@ -17,22 +13,28 @@ Module Rec.
   
   Fixpoint recdata (t : rectype) : Type := 
     match t with
-      | nil => unit
-      | (_, n) :: t' => word n * recdata t'
+    | nil => unit
+    | (_, l) :: t' => word l * recdata t'
     end%type.
 
+  Fixpoint reclen (t : rectype) : nat :=
+    match t with
+    | nil => 0
+    | (_, l) :: t' => l + reclen t'
+    end.
+
   Inductive field_in : rectype -> string -> Prop :=
-  | FE : forall t n w, field_in ((n, w) :: t) n
-  | FS : forall t n n' w, field_in t n -> field_in ((n',w) :: t) n.
+  | FE : forall t n l, field_in ((n, l) :: t) n
+  | FS : forall t n n' l, field_in t n -> field_in ((n', l) :: t) n.
 
   Lemma empty_field_in : forall n, ~(field_in nil n).
   Proof.
     intros n f. inversion f.
   Qed.
 
-  Lemma field_in_next : forall t n n' w, n' <> n -> field_in ((n',w) :: t) n -> field_in t n.
+  Lemma field_in_next : forall t n n' l, n' <> n -> field_in ((n',l) :: t) n -> field_in t n.
   Proof.
-    intros t n n' w ne f. inversion f; subst.
+    intros t n n' l ne f. inversion f; subst.
     contradiction ne. reflexivity.
     apply H3.
   Qed.
@@ -40,9 +42,9 @@ Module Rec.
   Fixpoint field_type (t : rectype) (n : string) (f : field_in t n) : nat :=
     match t as t return (field_in t n -> nat) with
     | nil => fun f => match (empty_field_in f) with end
-    | (n0, w0)::_ => fun f =>
+    | (n0, l0)::_ => fun f =>
       match (string_dec n0 n) with
-      | left _ => w0
+      | left _ => l0
       | right ne => field_type (field_in_next ne f)
       end
     end f.
@@ -50,13 +52,13 @@ Module Rec.
   Fixpoint recget (t : rectype) (n : string) (r : recdata t) (p : field_in t n) : word (field_type p) :=
     match t as t return (recdata t -> forall f : field_in t n, word (field_type f)) with
     | [] => fun _ f => match (empty_field_in f) with end
-    | (n0, w0) :: t' =>
+    | (n0, l0) :: t' =>
       fun r f =>
       let (v, r') := r in
       match (string_dec n0 n) as s
         return (word
             match s with
-            | left _ => w0
+            | left _ => l0
             | right ne => field_type (field_in_next ne f)
             end)
       with
@@ -81,15 +83,15 @@ Module Rec.
   Fixpoint fieldp (t : rectype) (n : string) : option (field_in t n) :=
     match t as t return (option (field_in t n)) with
     | [] => None
-    | (n0, w0) :: t' =>
+    | (n0, l0) :: t' =>
       match (string_dec n0 n) with
       | left e =>
           eq_rec_r
-            (fun n1 => option (field_in ((n1, w0) :: t') n))
-            (Some (FE t' n w0)) e
+            (fun n1 => option (field_in ((n1, l0) :: t') n))
+            (Some (FE t' n l0)) e
       | right _ =>
         match (fieldp t' n) with
-        | Some f => Some (FS n0 w0 f)
+        | Some f => Some (FS n0 l0 f)
         | None => None
         end
       end
@@ -104,7 +106,8 @@ Module Rec.
       | Some p => recget r p
       | None => I
     end.
-  
+  Notation "r :-> n" := (recget' n r) (at level 80).
+
   (* TODO 
   Definition recset' {t : rectype} {w : nat} (n : string) (r : recdata t) (v : word w) :=
     match fieldp t n as fp
@@ -119,13 +122,37 @@ Module Rec.
       | None => I
     end.
 *)
-  
-  Notation "r :-> n" := (recget' n r) (at level 80).
-  
+
+  Fixpoint rec2word {t : rectype} (r : recdata t) : word (reclen t) :=
+    match t as t return recdata t -> word (reclen t) with
+    | nil => fun _ => WO
+    | (_, _) :: _ => fun r =>
+      let (v, r') := r in combine v (rec2word r')
+    end r.
+
+  Fixpoint word2rec (t : rectype) (w : word (reclen t)) : recdata t :=
+    match t as t return word (reclen t) -> recdata t with
+    | nil => fun _ => tt
+    | (_, l) :: t' => fun w =>
+      (split1 l (reclen t') w, word2rec t' (split2 l (reclen t') w))
+    end w.
+
+  Theorem rec2word_word2rec : forall t w, rec2word (word2rec t w) = w.
+    induction t. auto.
+    intro w. destruct a as [n l]. simpl.
+    rewrite IHt. apply combine_split.
+  Qed.
+
+  Theorem word2rec_rec2word : forall t r, word2rec t (rec2word r) = r.
+    induction t; intro r.
+    destruct r. reflexivity.
+    destruct a as [n l]. destruct r. simpl.
+    rewrite split1_combine. rewrite split2_combine. rewrite IHt.
+    reflexivity.
+  Qed.
+
   Definition inodetype : rectype := [("free", 1); ("len", 16); ("block0", 16)].
   Definition inode1 : recdata inodetype := ($1, ($11, ($1677, tt))).
   Parameter inode2 : recdata inodetype.
   Definition foo := Eval compute in inode2 :-> "len".
-  Extraction Language Haskell.
-  Extraction foo.
 End Rec.
